Work on bounds

theories/L6_PCPS/Heap/compat.v
@@ -158,11 +158,11 @@ Module Compat (H : Heap).
       
     Definition InvGC :=
       forall (H1 H1' H2 H2' : heap block) (rho1 rho2 : env) (e1 e2 : exp)
-        B {Hf : ToMSet B} c1 c2 m1 m2 k,
-        IG k B  _ (H1', rho1, e1, c1, m1) (H2', rho2, e2, c2, m2) ->
+        S {Hs : ToMSet S} B {Hf : ToMSet B} c1 c2 m1 m2,
+        IG S _  B  _ (H1', rho1, e1, c1, m1) (H2', rho2, e2, c2, m2) ->
         live (env_locs rho1 (occurs_free e1)) H1 H1' ->
         live' (env_locs rho2 (occurs_free e2)) H2 H2' ->
-        IG k B _ (H1, rho1, e1, c1, m1) (H2, rho2, e2, c2, m2).
+        IG S _ B _ (H1, rho1, e1, c1, m1) (H2, rho2, e2, c2, m2).
 
     Definition IInvAppCompat (H1 H2 : heap block) (rho1 rho2 : env) f1 t xs1 f2 xs2 f2' Γ :=   
       forall (i  : nat) (H1' H1'' H2' : heap block)
@@ -179,7 +179,8 @@ Module Compat (H : Heap).
         injective_subdomain (reach' H2 (env_locs rho2 (occurs_free (AppClo clo_tag f2 t xs2 f2' Γ)))) β2 ->
 
         
-        IG i (name_in_fundefs B1) _ (H1'', rho_clo2, e1, c1, m1) (H2', rho2'', e2, c2, m2) ->
+        IG (FromList xs1) _ (name_in_fundefs B1) _
+           (H1'', rho_clo2, e1, c1, m1) (H2', rho2'', e2, c2, m2) ->
         IIL1 (H1', rho1', Eapp f1 t xs1) (H2', rho2', AppClo clo_tag f2 t xs2 f2' Γ) ->
         
         M.get f1 rho1' = Some (Loc l1) ->
